exercise 2 part b

FormaleSystemeInLean/LectureAndExercise/exercise2.lean
@@ -1,6 +1,6 @@
-import FormaleSystemeInLean.LectureAndExercise.lecture1
+import FormaleSystemeInLean.LectureAndExercise.lecture4
 
-
+/-
 structure DFA (Q : Type u) (Sigma : Type v) [Fintype Q] [Fintype Sigma] where
   δ: Q -> Sigma → Option Q
   q0 : Q
@@ -29,11 +29,11 @@ def NFA.Run.accepts {nfa : NFA Q Sigma} (_ : nfa.Run q qf w) : Prop := qf ∈ nf
 
 def NFA.Language (nfa : NFA Q Sigma) : Language Sigma :=
   fun w => ∃ (q0 qf : Q) (r : nfa.Run q0 qf w), r.from_start ∧ r.accepts
-
+-/
 
 section Exercise3
 
-  variable {Q1 : Type u1} {Q2 : Type u2} [Fintype Q1] [Fintype Q2]
+  variable {Sigma : Type u} {Q1 : Type u1} {Q2 : Type u2} [Fintype Q1] [Fintype Q2] [Fintype Sigma]
 
   structure NFASimulation (nfa1 : NFA Q1 Sigma) (nfa2 : NFA Q2 Sigma) where
     rel : Set (Q1 × Q2)
@@ -67,9 +67,234 @@ section Exercise3
       . exact r2_start
       . exact sim.final qf1_eq_qf2 r1_accept
 
-    theorem part_b : ∃ (nfa1 : NFA Q1 Sigma) (nfa2 : NFA Q2 Sigma), nfa1.Language ⊆ nfa2.Language ∧ ∀ (r : Set (Q1 × Q2)), ¬∃ (sim : NFASimulation nfa1 nfa2), sim.rel = r := by
 
-      sorry
+
+    def statesList := ["q0", "q1", "q2"]
+    def sigma := ['a', 'b']
+
+    def Q := { q : String // q ∈ statesList }
+    def ⅀ := { a : Char // a ∈ sigma }
+
+    instance : Fintype Q where
+      elems := statesList.attach
+      complete := by
+        intro q
+        rcases q with ⟨v, p⟩
+        unfold statesList at p
+        simp only [List.attach, Q, statesList, List.attachWith, List.pmap]
+        grind
+
+    instance : Fintype ⅀ where
+      elems := sigma.attach
+      complete := by
+        intro a
+        rcases a with ⟨v, p⟩
+        unfold sigma at p
+        simp only [List.attach, ⅀, sigma, List.attachWith, List.pmap]
+        grind
+
+    instance : BEq Q where
+      beq := fun q r => if q.val = r.val then true else false
+
+    instance : Fintype (Option Q) where
+      elems := statesList.attach.map (some · ) ++ [.none]
+      complete := by
+        intro q
+        simp --only [List.mem_map]
+        have some_mem (r : Q) : some r ∈ statesList.attach.map (some · ) ++ [.none] := by simp
+        by_cases hq : q = none
+        . apply Or.inr; exact hq
+        . rw [← Ne.eq_1, Option.ne_none_iff_exists] at hq
+          rcases hq with ⟨r, r_eq⟩
+          rcases r with ⟨v, p⟩
+          apply Or.inl
+          exists v, p
+
+    instance : Fintype (Set Q) := inferInstance
+
+    instance : Inter (Powertype Q) where
+      inter A B := fun e => e ∈ A ∧ e ∈ B
+
+    instance : BEq (Set Q) where
+      beq := sorry--fun X Y => if X = Y then true else false
+
+    instance : BEq (Powertype Q) := sorry
+
+    instance : LawfulBEq (Set Q) where
+      rfl := by sorry
+      eq_of_beq := sorry
+
+    instance : Fintype (Option (Powertype Q)) := sorry
+    instance : BEq (Set (Powertype Q)) := sorry
+    instance : DecidableEq (Powertype Q) := sorry
+
+    deriving instance DecidableEq for Q
+
+    def 𝓜 : NFA Q ⅀ where
+      δ := fun q σ =>
+        match q.val with
+          | "q0" => match σ.val with
+            | 'a' => [⟨"q2", by simp only [statesList]; grind⟩]
+            | 'b' => [⟨"q1", by simp only [statesList]; grind⟩, ⟨"q2", by simp only [statesList]; grind⟩]
+            | _ => []
+          | "q1" => match σ.val with
+            | 'b' => [⟨"q0", by simp only [statesList]; grind⟩, ⟨"q2", by simp only [statesList]; grind⟩]
+            | _ => []
+          | "q2" => []
+          | _ => []
+      Q0 := [⟨"q0", by simp only [statesList]; grind⟩]
+      F := [⟨"q2", by simp only [statesList]; grind⟩]
+
+    def 𝓜' : TotalDFA (Powertype Q) ⅀ := 𝓜.to_TotalDFA
+    def 𝓜'' : NFA (Powertype Q) ⅀ := 𝓜'.to_NFA
+
+    theorem part_b : ∃ (nfa1 : NFA (Powertype Q) ⅀) (nfa2 : NFA Q ⅀), nfa1.Language ⊆ nfa2.Language ∧ ∀ (r : Set ((Powertype Q) × Q)), ¬∃ (sim : NFASimulation nfa1 nfa2), sim.rel = r := by
+      exists 𝓜'', 𝓜
+      constructor
+      . intro w w_mem
+        have lang_eq1 : 𝓜.to_TotalDFA.Language = 𝓜.Language := by
+          apply NFA_totalDFA_lang_eq 𝓜
+        have lang_eq2 : 𝓜''.Language = 𝓜'.Language := by
+          unfold 𝓜''
+          apply totalDFA_NFA_lang_eq 𝓜'
+        unfold 𝓜'' 𝓜' at *
+        rw [← lang_eq2] at lang_eq1
+        rw [← lang_eq1]
+        exact w_mem
+      . intro rel
+        intro contra
+        rcases contra with ⟨sim, sim_eq⟩
+        rcases sim with ⟨sim, start, step, final⟩
+
+        have q01_mem : (fun q => q = ⟨"q0", by simp only [statesList]; grind⟩) ∈ 𝓜''.Q0 := by
+          unfold 𝓜'' TotalDFA.to_NFA 𝓜' 𝓜 NFA.to_TotalDFA List.toSet
+          simp
+        have q02_mem : ⟨"q0", by simp only [statesList]; grind⟩ ∈ 𝓜.Q0 := by unfold 𝓜; simp
+        have q02_eq : 𝓜.Q0 = [⟨"q0", by simp only [statesList]; grind⟩] := by unfold 𝓜; simp
+
+        have start_mem : sim (fun q => q = ⟨"q0", by simp only [statesList]; grind⟩, ⟨"q0", by simp only [statesList]; grind⟩) := by
+          have aux := start (fun q => q = ⟨"q0", by simp only [statesList]; grind⟩) q01_mem
+          rcases aux with ⟨q02, q02_mem', mem_sim⟩
+          rw [q02_eq, List.mem_singleton] at q02_mem'
+          rw [q02_mem'] at mem_sim
+          exact mem_sim
+
+        have delta'_q0_eq : 𝓜''.δ (fun q => q = ⟨"q0", by simp only [statesList]; grind⟩) ⟨'b', by simp only [sigma]; grind⟩ = [(fun q => q = ⟨"q1", by simp only [statesList]; grind⟩ ∨ q = ⟨"q2", by simp only [statesList]; grind⟩)] := by
+          unfold 𝓜'' TotalDFA.to_NFA 𝓜' 𝓜 NFA.to_TotalDFA List.toSet
+          simp
+          apply funext
+          intro x
+          apply propext
+          constructor
+          . intro hr
+            rcases hr with ⟨r, r_mem, x_mem⟩
+            simp only [Membership.mem] at r_mem
+            simp only [r_mem] at x_mem
+            simp at x_mem
+            exact x_mem
+          . intro x_eq
+            exists ⟨"q0", by simp only [statesList]; grind⟩
+            constructor
+            . simp only [Membership.mem]
+            . simp
+              exact x_eq
+
+        have delta_q0_eq : 𝓜.δ ⟨"q0", by simp only [statesList]; grind⟩ ⟨'b', by simp only [sigma]; grind⟩ = [⟨"q1", by simp only [statesList]; grind⟩, ⟨"q2", by simp only [statesList]; grind⟩] := by simp only [𝓜]
+
+        have mem_step : sim ((fun q => q = ⟨"q1", by simp only [statesList]; grind⟩ ∨ q = ⟨"q2", by simp only [statesList]; grind⟩), ⟨"q2", by simp only [statesList]; grind⟩) := by
+          have aux := step (a := ⟨'b', by simp only [sigma]; grind⟩) start_mem
+          have mem_delta : (fun q => q = ⟨"q1", by simp only [statesList]; grind⟩ ∨ q = ⟨"q2", by simp only [statesList]; grind⟩) ∈ 𝓜''.δ (fun q => q = ⟨"q0", by simp only [statesList]; grind⟩) ⟨'b', by simp only [sigma]; grind⟩ := by grind
+          specialize aux (fun q => q = ⟨"q1", by simp only [statesList]; grind⟩ ∨ q = ⟨"q2", by simp only [statesList]; grind⟩)
+          have aux2 := aux mem_delta
+          rcases aux2 with ⟨r, r_mem, mem_sim⟩
+          rw [delta_q0_eq] at r_mem
+
+          have nmem_q1 : ¬sim ((fun q => q = ⟨"q1", by simp only [statesList]; grind⟩ ∨ q = ⟨"q2", by simp only [statesList]; grind⟩), ⟨"q1", by simp only [statesList]; grind⟩) := by
+            intro contra
+            have mem_F : (fun q => q = ⟨"q1", by simp only [statesList]; grind⟩ ∨ q = ⟨"q2", by simp only [statesList]; grind⟩) ∈ 𝓜''.F := by
+              simp only [𝓜'', TotalDFA.to_NFA, 𝓜', NFA.to_TotalDFA, List.mem_filter, Fintype.elems, List.mem_map]
+              constructor
+              . sorry
+              . unfold 𝓜 List.toSet
+                simp
+                intro contra'
+                let X : (Powertype Q) := (fun e => e = ⟨"q2", by simp only [statesList]; grind⟩)
+                let Y : (Powertype Q) := fun q => q = ⟨"q1", by simp only [statesList]; grind⟩ ∨ q = ⟨"q2", by simp only [statesList]; grind⟩
+                have inter : X ∩ Y = (fun q => q = ⟨"q2", by simp only [statesList]; grind⟩) := by
+                  apply Set.ext
+                  intro t
+                  constructor
+                  . intro t_mem
+                    rcases t_mem with ⟨l, r⟩
+                    simp only [X, Y, Membership.mem] at *
+                    grind
+                  . intro t_mem
+                    simp only [Membership.mem] at t_mem
+                    constructor
+                    . simp only [X, Membership.mem]; exact t_mem
+                    . simp only [Y, Membership.mem]; apply Or.inr; exact t_mem
+                simp only [X, Y] at inter
+                rw [Set.empty_iff] at contra'
+                have nmem := contra' ⟨"q2", by simp only [statesList]; grind⟩
+                have mem : ⟨"q2", by simp only [statesList]; grind⟩ ∈ X ∩ Y := by
+                  simp only [X, Y, inter]
+                  simp only [Membership.mem]
+                simp only [X, Y] at mem
+                contradiction
+
+            have aux3 := final contra mem_F
+            simp only [𝓜, List.mem_singleton] at aux3
+            contradiction
+
+          have r_neq : ¬r = ⟨"q1", by simp only [statesList]; grind⟩ := by
+            intro contra
+            rw [contra] at mem_sim
+            contradiction
+          have r_eq : r = ⟨"q2", by simp only [statesList]; grind⟩ := by
+            simp at r_mem
+            grind
+
+          rw [r_eq] at mem_sim
+          exact mem_sim
+
+        have delta_undef : ∀ (a : ⅀), ¬∃ r, r ∈ 𝓜.δ ⟨"q2", by simp only [statesList]; grind⟩ a := by
+          intro a contra
+          rcases contra with ⟨r, r_mem⟩
+          simp only [𝓜] at r_mem
+          simp_all
+
+        have delta_q1_q2 : (fun q => q = ⟨"q0", by simp only [statesList]; grind⟩ ∨ q = ⟨"q2", by simp only [statesList]; grind⟩) ∈ 𝓜''.δ (fun q => q = ⟨"q1", by simp only [statesList]; grind⟩ ∨ q = ⟨"q2", by simp only [statesList]; grind⟩) ⟨'b', by simp only [sigma]; grind⟩ := by
+          simp only [𝓜'', TotalDFA.to_NFA, 𝓜', NFA.to_TotalDFA, 𝓜]
+          simp
+          apply Set.ext
+          intro q
+          constructor
+          . intro q_mem
+            simp only [Membership.mem]
+            exists ⟨"q1", by simp only [statesList]; grind⟩
+            constructor
+            . apply Or.inl; rfl
+            . simp only [Membership.mem] at q_mem
+              simp
+              by_cases hq : q = ⟨"q0", by simp only [statesList]; grind⟩
+              . rw [hq]
+
+                sorry
+              . simp only [hq, false_or] at q_mem
+                rw [q_mem]
+                constructor
+
+                sorry
+          . intro q_mem
+            rcases q_mem with ⟨r, r_mem, q_mem⟩
+            simp only [Membership.mem] at *
+
+            sorry
+
+        have mem_step2 := step (a := ⟨'b', by simp only [sigma]; grind⟩) mem_step (fun q => q = ⟨"q0", by simp only [statesList]; grind⟩ ∨ q = ⟨"q2", by simp only [statesList]; grind⟩) delta_q1_q2
+        rcases mem_step2 with ⟨r, r_mem, mem_sim⟩
+        specialize delta_undef ⟨'b', by simp only [sigma]; grind⟩
+        contradiction
 
   end d
 
